progress

main-results/VCGEndToEnd.thy
@@ -4,6 +4,48 @@ begin
 
 section \<open>Theorem VCG back-end to ViperCore operational semantics\<close>
 
+
+subsection \<open>Helper\<close>
+
+fun valid_front_end_cmd :: "cmd \<Rightarrow> bool"
+  where
+    "valid_front_end_cmd (Cseq C1 C2) \<longleftrightarrow> valid_front_end_cmd C1 \<and> valid_front_end_cmd C2"
+  | "valid_front_end_cmd ({P1} C1 {P2} || {Q1} C2 {Q2})  \<longleftrightarrow> valid_a2t_assert P1 \<and> valid_a2t_assert P2
+                                                          \<and> valid_a2t_assert Q1 \<and> valid_a2t_assert Q2 \<and>
+                                                            valid_front_end_cmd C1 \<and> valid_front_end_cmd C2"
+  | "valid_front_end_cmd (Cif B C1 C2) \<longleftrightarrow> valid_front_end_cmd C1 \<and> valid_front_end_cmd C2"
+  | "valid_front_end_cmd (Cwhile B I C)    \<longleftrightarrow> valid_a2t_assert I \<and> valid_front_end_cmd C"
+  | "valid_front_end_cmd _    = True"
+
+lemma valid_a2t_exp_translate_exp: "valid_a2t_exp (translate_exp e)"
+  by (induction e) auto
+
+lemma valid_a2t_bexp_translate_exp: "valid_a2t_exp (translate_bexp e)"
+  apply (induction e)
+  using valid_a2t_exp_translate_exp
+  by auto
+
+lemma vald_a2t_stmt_n_havoc: "valid_a2t_stmt (n_havoc xs)"
+  by (induction xs) auto
+  
+lemma valid_a2t_stmt_translate_syn:
+  assumes "valid_front_end_cmd C"
+  shows "valid_a2t_stmt (fst (translate_syn \<Delta> t C)) \<and> (\<forall>aux \<in> snd (translate_syn \<Delta> t C). valid_a2t_stmt aux)"
+  using assms
+  apply (induction C)
+  apply (simp_all add: valid_a2t_exp_translate_exp 
+                      syntactic_translate_heap_loc_def
+                      syntactic_translate_addr_def
+                      Let_def 
+                      vald_a2t_stmt_n_havoc
+                      valid_a2t_bexp_translate_exp)
+    apply fastforce
+   apply blast
+  apply blast
+  done
+
+subsection \<open>Main\<close>
+
 definition triple_as_method_decl :: "vtyp list \<Rightarrow> ViperLang.assertion \<Rightarrow> stmt \<Rightarrow> ViperLang.assertion \<Rightarrow> method_decl"
   where "triple_as_method_decl ts P C Q \<equiv> \<lparr> method_decl.args = [], 
                                          rets = ts, 
@@ -94,7 +136,9 @@ corollary VCG_to_verifies_set :
   assumes MethodCorrect: "vpr_method_correct_total ctxt (\<lambda>_ :: int full_total_state. True) (triple_as_method_decl ts P C Q)"
       and "\<Lambda> = nth_option ts"
       and Typed: "stmt_typing (program_total ctxt) \<Lambda> (stmt.Seq (stmt.Seq (stmt.Inhale P) C) (stmt.Exhale Q))"
-      and "valid_a2t_stmt C"
+      and ValidC: "valid_a2t_stmt C"
+      and ValidPre: "valid_a2t_assert P"
+      and ValidPost: "valid_a2t_assert Q"
       and AbsTypeWf: "abs_type_wf (absval_interp_total ctxt)"
     shows "ConcreteSemantics.verifies_set (t2a_ctxt ctxt \<Lambda>) (initial_vcg_states_equi (t2a_ctxt ctxt \<Lambda>))
             (compile False (ctxt_to_interp ctxt) (\<Lambda>, declared_fields (program_total ctxt)) 
@@ -196,25 +240,11 @@ next
     by (simp add: AbsTypeWf)
 next
   show "valid_a2t_stmt (stmt.Seq (stmt.Seq (stmt.Inhale P) C) (stmt.Exhale Q))"
-    sorry
-qed    
-
-lemma valid_a2t_exp_translate_exp: "valid_a2t_exp (translate_exp e)"
-  by (induction e) auto
-
-lemma valid_a2t_stmt_translate_syn:
-  assumes "res = translate_syn \<Delta> t C"
-  shows "valid_a2t_stmt (fst res)"
-  using assms
-  (*apply (induction C)
-           apply (simp_all add: valid_a2t_exp_translate_exp 
-                                syntactic_translate_heap_loc_def
-                                syntactic_translate_addr_def)*)
-  oops 
+    by (simp add: ValidC ValidPre ValidPost)
+qed 
 
 abbreviation true_syn_assertion 
   where "true_syn_assertion \<equiv> (Atomic (Pure (ELit (LBool True))))"
-
 
 lemma custom_context_tcfe_eq:
   "custom_context tcfe =
@@ -233,6 +263,8 @@ theorem sound_syntactic_translation_VCG:
       and "\<And>Cv. Cv \<in> snd (translate \<Delta> C) \<Longrightarrow> ConcreteSemantics.wf_abs_stmt tcfe Cv"
       and "TypedEqui.wf_assertion tcfe P \<and> TypedEqui.wf_assertion tcfe Q"
       and "typed_stmt C" (* TODO: Unify the two notions of typing *)
+      and ValidFrontendCmd: "valid_front_end_cmd C"
+      and ValidPrePost: "valid_a2t_assert Ps \<and> valid_a2t_assert Qs"
 
       and AbsTypeWf: "abs_type_wf (interp.domains \<Delta>)"
       and InterpFunsPredsEmpty: "interp.funs \<Delta> = (\<lambda> _ _ _. None) \<and> interp.predicates \<Delta> = Map.empty"
@@ -276,9 +308,9 @@ proof (rule sound_syntactic_translation[OF assms(1-6)], simp)
       using ViperTyped
       unfolding \<open>mdecl = _\<close>
         apply blast
-       defer
-      apply (simp add: default_ctxt_def AbsTypeWf)
-      sorry
+      using valid_a2t_stmt_translate_syn[OF ValidFrontendCmd]
+       apply fast
+      by (simp_all add: default_ctxt_def AbsTypeWf ValidPrePost)
 
     have "ConcreteSemantics.verifies_set tcfe (initial_vcg_states_equi (t2a_ctxt ?ctxt ?\<Lambda>)) (compile False \<Delta> tcfes ?Ctr_mainV)"
     proof -
@@ -343,9 +375,9 @@ proof (rule sound_syntactic_translation[OF assms(1-6)], simp)
          apply blast
         apply simp
         apply (rule TypingAux)
-       defer
-       apply (simp add: default_ctxt_def AbsTypeWf)
-      sorry
+       using valid_a2t_stmt_translate_syn[OF ValidFrontendCmd] \<open>Cv_syn \<in> _\<close>
+       apply fast      
+       by (simp_all add: default_ctxt_def AbsTypeWf ValidPrePost)
 
     hence A1: "ConcreteSemantics.verifies_set (t2a_ctxt ?ctxt ?\<Lambda>) (initial_vcg_states_equi (t2a_ctxt ?ctxt ?\<Lambda>))
                (compile False (ctxt_to_interp ?ctxt) (?\<Lambda>, declared_fields (program_total ?ctxt)) Cv_syn)"
